Prove success for quicksort monadic translator example

translator/monadic/examples/polyArraySortProgScript.sml
@@ -33,6 +33,47 @@ val _ = start_translation config;
 
 (*******************************************************************************
 
+    TODO MOVE TO ml_monadBaseTheory
+
+*******************************************************************************)
+
+Theorem Msub_Success:
+  ∀ l n e x . (Msub e n l = Success x) ⇔ n < LENGTH l ∧ (x = EL n l)
+Proof
+  Induct >>
+  simp[Once ml_monadBaseTheory.Msub_def] >>
+  rw[]
+  >- (EQ_TAC >> rw[]) >>
+  Cases_on `n` >> fs[] >>
+  EQ_TAC >> rw[]
+QED
+
+Theorem Mupdate_Success:
+  ∀ l n x e res . (Mupdate e x n l = Success res)
+  ⇔ (n < LENGTH l ∧ (res = LUPDATE x n l))
+Proof
+  rw[] >>
+  EQ_TAC >>
+  rw[]
+  >- (
+    CCONTR_TAC >>
+    fs[NOT_LESS] >>
+    qspecl_then [`l`,`n`,`x`,`e`] assume_tac
+      ml_monadBaseTheory.Mupdate_exn_eq  >>
+    fs[]
+    )
+  >- (
+    Cases_on `n < LENGTH l` >> fs[ml_monadBaseTheory.Mupdate_exn_eq] >>
+    fs[ml_monadBaseTheory.Mupdate_eq]
+  )
+  >- (
+    fs[ml_monadBaseTheory.Mupdate_eq]
+    )
+QED
+
+
+(*******************************************************************************
+
     ARRAY SETTERS AND GETTERS
 
 *******************************************************************************)
@@ -79,18 +120,6 @@ val array_get_v_thm = m_translate array_get_def;
     SCAN_UPPER / SCAN_LOWER
 
 *******************************************************************************)
-
-(* TODO move to ml_monadBaseTheory *)
-Theorem Msub_Success:
-  ∀ l n e x . (Msub e n l = Success x) ⇔ n < LENGTH l ∧ (x = EL n l)
-Proof
-  Induct >>
-  simp[Once ml_monadBaseTheory.Msub_def] >>
-  rw[]
-  >- (EQ_TAC >> rw[]) >>
-  Cases_on `n` >> fs[] >>
-  EQ_TAC >> rw[]
-QED
 
 val scan_lower_def = mtDefine "scan_lower" `
   scan_lower (cmp : 'a -> 'a -> bool) pivot lb = do
@@ -330,30 +359,38 @@ val _ = UNDISCH_ALL partition_helper_v_thm_precond_thm |>
 Theorem partition_helper_index:
   ∀ cmp pivot lb ub s p s' .
     ub > lb ∧ (partition_helper cmp pivot lb ub s = (Success p, s'))
-  ⇒ p ≥ lb
+  ⇒ p ≥ lb ∧ p ≤ ub
 Proof
   recInduct (theorem "partition_helper_ind") >>
-  rw[] >>
-  qpat_x_assum `partition_helper _ _ _ _ _ = _` mp_tac >>
+  rpt gen_tac >> strip_tac >> rpt gen_tac >>
   simp[Once partition_helper_def] >>
   fs[ml_monadBaseTheory.st_ex_bind_def,
      ml_monadBaseTheory.st_ex_ignore_bind_def] >>
-  EVERY_CASE_TAC >> fs[]
+  EVERY_CASE_TAC >> fs[] >>
+  rename1 `scan_lower _ _ _ _ = (Success new_lb, _)` >>
+  rename1 `scan_upper _ _ _ _ = (Success new_ub, _)`
     >- (
-      rw[] >>
+      strip_tac >>
       imp_res_tac scan_lower_index >>
-      qsuff_tac `p >= a'` >- fs[] >>
+      imp_res_tac scan_upper_index >> fs[prim_recTheory.NOT_LESS_0] >>
+      qsuff_tac `p ≥ new_lb ∧ p ≤ new_ub` >- fs[] >>
       qpat_x_assum `partition_helper _ _ _ _ _ = _ ` mp_tac >>
       first_assum match_mp_tac >>
       fs[]
       )
     >- (
       fs[ml_monadBaseTheory.st_ex_return_def] >>
-      rw[] >>
+      strip_tac >>
       fs[NOT_LESS] >>
+      rveq >>
       imp_res_tac scan_lower_index >>
       imp_res_tac scan_upper_index >> fs[prim_recTheory.NOT_LESS_0]
-      metis_tac[]
+      drule scan_lower_state >>
+      strip_tac >> rveq >>
+      drule scan_upper_state >>
+      strip_tac >> rveq >>
+      Cases_on `new_ub = new_lb` >> fs[] >>
+      cheat
       )
 QED
 *)
@@ -438,6 +475,363 @@ val run_quicksort_def = Define `
 `;
 
 val run_quicksort_v_thm = m_translate_run run_quicksort_def;
+
+
+(*******************************************************************************
+
+    PROOF OF SUCCESS
+
+*******************************************************************************)
+
+(* borrowed from examples/quicksortProg *)
+val strict_weak_order_def = Define `
+  strict_weak_order r ⇔
+    transitive r ∧
+    (∀ x y. r x y ⇒ ¬ r y x) ∧
+    transitive (λ x y. ¬ r x y ∧ ¬ r y x)`;
+
+Theorem strict_weak_order_alt:
+  ∀ r . strict_weak_order r ⇔
+    (∀ x y. r x y ⇒ ¬ r y x) ∧
+    transitive (λ x y. ¬ r y x)
+Proof
+  rw [strict_weak_order_def, transitive_def] >>
+  metis_tac []
+QED
+
+Theorem strict_weak_order_irreflexive:
+  ∀ r . strict_weak_order r ⇒ irreflexive r
+Proof
+  rw[irreflexive_def] >>
+  fs[strict_weak_order_def] >>
+  metis_tac[]
+QED
+
+Theorem scan_lower_Success:
+  ∀ cmp pivot lb s .
+    strict_weak_order cmp ∧ lb < LENGTH s.arr ∧
+    (∃ index . index ≥ lb ∧ index < LENGTH s.arr ∧ (EL index s.arr = pivot))
+  ⇒ ∃ result s' . (scan_lower cmp pivot lb s = (Success result, s'))
+Proof
+  recInduct (theorem "scan_lower_ind") >>
+  rw[] >>
+  simp[Once scan_lower_def] >>
+  fs[ml_monadBaseTheory.st_ex_bind_def, ml_monadBaseTheory.st_ex_return_def] >>
+  EVERY_CASE_TAC >> fs[]
+  >- (
+      fs[fetch "-" "arr_sub_def", ml_monadBaseTheory.Marray_sub_def] >>
+      rveq >>
+      Cases_on `index = lb` >> fs[]
+      >- (
+        imp_res_tac Msub_Success >>
+        imp_res_tac strict_weak_order_irreflexive >>
+        rveq >>
+        fs[irreflexive_def]
+        ) >>
+      first_x_assum match_mp_tac >>
+      fs[] >>
+      qexists_tac `index` >> fs[]
+    )
+  >- (
+    fs[fetch "-" "arr_sub_def", ml_monadBaseTheory.Marray_sub_def] >>
+    rveq >>
+    `lb < LENGTH r.arr` by fs[] >>
+    imp_res_tac (Msub_Success |> INST_TYPE [beta |-> ``:state_exn``]) >>
+    fs[]
+    )
+QED
+
+Theorem scan_upper_Success:
+  ∀ cmp pivot ub s .
+    ub ≤ LENGTH s.arr
+  ⇒ ∃ result s' . (scan_upper cmp pivot ub s = (Success result, s'))
+Proof
+  recInduct (theorem "scan_upper_ind") >>
+  rw[] >>
+  simp[Once scan_upper_def] >>
+  fs[ml_monadBaseTheory.st_ex_bind_def, ml_monadBaseTheory.st_ex_return_def] >>
+  fs[fetch "-" "arr_sub_def", ml_monadBaseTheory.Marray_sub_def] >>
+  EVERY_CASE_TAC >> fs[]
+  >- (
+    first_x_assum drule >>
+    strip_tac >>
+    first_x_assum match_mp_tac >>
+    fs[]
+    )
+  >- (
+      `ub - 1 < LENGTH s.arr` by fs[] >>
+      imp_res_tac
+        (ml_monadBaseTheory.Msub_eq |> INST_TYPE [beta |-> ``:state_exn``]) >>
+      fs[]
+    )
+QED
+
+Theorem partition_helper_Success:
+  ∀ cmp pivot lb ub s .
+    strict_weak_order cmp ∧
+    ub ≤ LENGTH s.arr ∧
+    (∃ index . index ≥ lb ∧ index < LENGTH s.arr ∧ (EL index s.arr = pivot))
+  ⇒ ∃ result s' . partition_helper cmp pivot lb ub s = (Success result, s')
+Proof
+  recInduct (theorem "partition_helper_ind") >>
+  rw[] >>
+  simp[Once partition_helper_def] >>
+  fs[ml_monadBaseTheory.st_ex_bind_def, ml_monadBaseTheory.st_ex_return_def,
+     ml_monadBaseTheory.st_ex_ignore_bind_def] >>
+  fs[fetch "-" "arr_sub_def", ml_monadBaseTheory.Marray_sub_def] >>
+  fs[fetch "-" "update_arr_def", ml_monadBaseTheory.Marray_update_def] >>
+  IF_CASES_TAC >> fs[NOT_LEQ, ADD1] >>
+  qspecl_then [`cmp`,`EL index s.arr`,`lb`,`s`] assume_tac scan_lower_Success >>
+  rfs[] >> first_x_assum imp_res_tac >> rfs[] >>
+  imp_res_tac scan_lower_state >> rveq >> fs[] >>
+  qspecl_then [`cmp`,`EL index s.arr`,`ub`,`s`] assume_tac scan_upper_Success >>
+  rfs[] >>
+  imp_res_tac scan_upper_state >> rveq >> fs[] >>
+  rename1 `scan_lower _ _ _ _ = (Success new_lb, _)` >>
+  rename1 `scan_upper _ _ _ _ = (Success new_ub, _)` >>
+  imp_res_tac scan_lower_index >>
+  imp_res_tac scan_upper_index >> fs[] >>
+  Cases_on `new_ub = 0` >> fs[] >>
+  IF_CASES_TAC >> fs[] >>
+  `new_lb < LENGTH s.arr` by fs[] >>
+  `new_ub < LENGTH s.arr` by fs[] >>
+  imp_res_tac (Msub_Success |> INST_TYPE [beta |-> ``:state_exn``]) >> fs[] >>
+  ntac 3 (first_x_assum (qspec_then `Subscript` mp_tac) >> strip_tac >> fs[]) >>
+  qspecl_then [`s.arr`,`new_lb`,`EL new_ub s.arr`,`Subscript`] assume_tac
+    (Mupdate_Success |> INST_TYPE [beta |-> ``:state_exn``]) >> fs[] >>
+  first_x_assum (qspec_then `LUPDATE (EL new_ub s.arr) new_lb s.arr` mp_tac) >>
+  fs[] >> strip_tac >> fs[] >>
+  qspecl_then [`LUPDATE (EL new_ub s.arr) new_lb s.arr`,
+               `new_ub`,`EL new_lb s.arr`,`Subscript`] assume_tac
+    (Mupdate_Success |> INST_TYPE [beta |-> ``:state_exn``]) >> fs[] >>
+  first_x_assum (qspec_then
+    `LUPDATE (EL new_lb s.arr) new_ub (LUPDATE (EL new_ub s.arr) new_lb s.arr)`
+      mp_tac) >>
+  fs[] >> strip_tac >> fs[] >>
+  first_x_assum match_mp_tac >>
+  fs[] >>
+  Cases_on `new_lb = index` >> fs[]
+  >- (
+    rveq >>
+    qexists_tac `new_ub` >> fs[EL_LUPDATE]
+    ) >>
+  Cases_on `new_ub = index` >> fs[]
+  >- (
+    rveq >>
+    qexists_tac `new_lb` >> fs[EL_LUPDATE]
+    ) >>
+  qexists_tac `index` >> fs[EL_LUPDATE] >>
+  last_x_assum (qspec_then `index` mp_tac) >>
+  Cases_on `index < new_lb` >> fs[] >>
+  metis_tac[strict_weak_order_irreflexive, irreflexive_def]
+QED
+
+Theorem partition_helper_state_LENGTH:
+  ∀ cmp pivot lb ub s result s'.
+    (partition_helper cmp pivot lb ub s = (Success result, s'))
+  ⇒ (LENGTH s'.arr = LENGTH s.arr)
+Proof
+  recInduct (theorem "partition_helper_ind") >>
+  rpt gen_tac >> strip_tac >> rpt gen_tac >>
+  simp[Once partition_helper_def] >>
+  fs[ml_monadBaseTheory.st_ex_bind_def, ml_monadBaseTheory.st_ex_return_def,
+     ml_monadBaseTheory.st_ex_ignore_bind_def] >>
+  fs[fetch "-" "arr_sub_def", ml_monadBaseTheory.Marray_sub_def] >>
+  fs[fetch "-" "update_arr_def", ml_monadBaseTheory.Marray_update_def] >>
+  EVERY_CASE_TAC >> fs[] >>
+  imp_res_tac scan_lower_state >>
+  imp_res_tac scan_upper_state >> rveq >> fs[] >>
+  rw[] >>
+  first_x_assum drule >>
+  rpt (disch_then drule) >>
+  rw[] >>
+  first_x_assum drule >>
+  fs[] >> rw[] >>
+  imp_res_tac Mupdate_Success >>
+  fs[LUPDATE_LENGTH]
+QED
+
+Theorem quicksort_aux_Success:
+  ∀ cmp lower upper s .
+    strict_weak_order cmp ∧
+    upper < LENGTH s.arr
+  ⇒ ∃ results s' . (quicksort_aux cmp lower upper s = (Success result, s')) ∧
+    (LENGTH s'.arr = LENGTH s.arr)
+Proof
+  recInduct (theorem "quicksort_aux_ind") >>
+  rw[] >>
+  simp[Once quicksort_aux_def] >>
+  fs[ml_monadBaseTheory.st_ex_bind_def, ml_monadBaseTheory.st_ex_return_def,
+     ml_monadBaseTheory.st_ex_ignore_bind_def] >>
+  fs[fetch "-" "arr_sub_def", ml_monadBaseTheory.Marray_sub_def] >>
+  IF_CASES_TAC >> fs[NOT_GREATER_EQ, ADD1, LE_LT1] >>
+  `lower < LENGTH s.arr` by fs[] >>
+  imp_res_tac (Msub_Success |> INST_TYPE [beta |-> ``:state_exn``]) >> fs[] >>
+  ntac 2 (first_x_assum (qspec_then `Subscript` mp_tac) >> strip_tac >> fs[]) >>
+  qspecl_then [`cmp`,`EL lower s.arr`,`lower`,`upper + 1`,`s`]
+    assume_tac partition_helper_Success >> rfs[] >>
+  (* TODO why do we have to manually state the below? *)
+  `∃ result s' . partition_helper cmp (EL lower s.arr) lower (upper + 1) s =
+    (Success result, s')` by
+      (first_x_assum match_mp_tac >> qexists_tac `lower` >> fs[]) >>
+  fs[] >>
+  reverse (IF_CASES_TAC) >> fs[]
+  >- metis_tac[partition_helper_state_LENGTH]
+  >- metis_tac[partition_helper_state_LENGTH]
+  >>
+  `∃ s . (quicksort_aux cmp lower result s' = (Success (), s)) ∧
+    (LENGTH s.arr = LENGTH s'.arr)` by (
+      first_x_assum match_mp_tac >>
+      imp_res_tac partition_helper_state_LENGTH >>
+      DECIDE_TAC) >>
+  fs[] >>
+  qsuff_tac `upper < LENGTH s'.arr`
+  >- (
+    rw[] >> fs[] >>
+    metis_tac[partition_helper_state_LENGTH]
+    ) >>
+  imp_res_tac partition_helper_state_LENGTH >>
+  DECIDE_TAC
+QED
+
+Theorem array_set_aux_Success:
+  ∀ l n s . (LENGTH (DROP n s.arr) = LENGTH l)
+  ⇒ ∃ s' . (array_set_aux n l s = (Success (), s')) ∧
+    (LENGTH s.arr = LENGTH s'.arr)
+Proof
+  Induct >>
+  rw[] >>
+  simp[Once array_set_aux_def] >>
+  fs[ml_monadBaseTheory.st_ex_ignore_bind_def,
+     ml_monadBaseTheory.st_ex_return_def] >>
+  fs[fetch "-" "update_arr_def", ml_monadBaseTheory.Marray_update_def] >>
+  fs[ADD1] >> rveq >>
+  qspecl_then [`s.arr`,`n`,`h`,`Subscript`] assume_tac
+    (Mupdate_Success |> INST_TYPE [beta |-> ``:state_exn``]) >> fs[] >>
+  first_x_assum (qspec_then `LUPDATE h n s.arr` mp_tac) >> strip_tac >> fs[] >>
+  fs[EQ_IMP_THM] >>
+  first_x_assum (qspecl_then [
+    `n + 1`, `<| arr := LUPDATE h n s.arr |>`] mp_tac) >>
+  fs[]
+QED
+
+(* TODO
+Theorem array_set_aux_Success:
+  ∀ l n s . (LENGTH (DROP n s.arr) = LENGTH l)
+  ⇒ ∃ s' . (array_set_aux n l s = (Success (), s')) ∧ (DROP n s'.arr = l)
+Proof
+  Induct >>
+  rw[] >>
+  simp[Once array_set_aux_def] >>
+  fs[ml_monadBaseTheory.st_ex_ignore_bind_def,
+     ml_monadBaseTheory.st_ex_return_def] >>
+  fs[fetch "-" "update_arr_def", ml_monadBaseTheory.Marray_update_def] >>
+  fs[ADD1] >> rveq
+  >- (qspecl_then [`s.arr`, `n`] assume_tac DROP_LENGTH_TOO_LONG >> fs[]) >>
+  qspecl_then [`s.arr`,`n`,`h`,`Subscript`] assume_tac
+    (Mupdate_Success |> INST_TYPE [beta |-> ``:state_exn``]) >> fs[] >>
+  first_x_assum (qspec_then `LUPDATE h n s.arr` mp_tac) >> strip_tac >> fs[] >>
+  fs[EQ_IMP_THM] >>
+  first_x_assum (qspecl_then [
+    `n + 1`, `<| arr := LUPDATE h n s.arr |>`] mp_tac) >>
+  fs[] >>
+  rw[] >>
+  qexists_tac `s'` >> fs[] >>
+  Cases_on `s'.arr` >> fs[] >>
+QED
+*)
+
+Theorem array_set_Success:
+  ∀ l s . (LENGTH l = LENGTH s.arr)
+  ⇒ ∃ s' . (array_set l s = (Success (), s')) ∧ (LENGTH s.arr = LENGTH s'.arr)
+Proof
+  rw[] >>
+  fs[array_set_def] >>
+  qspecl_then [`l`,`0n`,`s`] assume_tac array_set_aux_Success >>
+  fs[] >>
+  metis_tac[]
+QED
+
+Theorem array_get_aux_Success:
+  ∀ length n s . (LENGTH s.arr = length)
+  ⇒ ∃ result . (array_get_aux length n s = (Success result, s)) ∧
+    (result = DROP n s.arr)
+Proof
+  recInduct (theorem "array_get_aux_ind") >>
+  rw[] >>
+  simp[Once array_get_aux_def] >>
+  fs[ml_monadBaseTheory.st_ex_bind_def, ml_monadBaseTheory.st_ex_return_def,
+     ml_monadBaseTheory.st_ex_ignore_bind_def] >>
+  fs[fetch "-" "arr_sub_def", ml_monadBaseTheory.Marray_sub_def] >>
+  IF_CASES_TAC >> fs[]
+  >- (qspecl_then [`s.arr`, `n`] assume_tac DROP_LENGTH_TOO_LONG >> fs[]) >>
+  first_x_assum (qspec_then `s` mp_tac) >> strip_tac >> fs[] >>
+  fs[NOT_GREATER_EQ, ADD1, LE_LT1] >>
+  imp_res_tac (Msub_Success |> INST_TYPE [beta |-> ``:state_exn``]) >>
+  fs[] >>
+  fs[DROP_EL_CONS]
+QED
+
+Theorem array_get_Success:
+  ∀ s . ∃ s' . array_get () s = (Success s.arr, s)
+Proof
+  simp[Once array_get_def] >>
+  fs[ml_monadBaseTheory.st_ex_bind_def] >>
+  fs[fetch "-" "arr_length_def", ml_monadBaseTheory.Marray_length_def] >>
+  rw[] >>
+  qspecl_then [`LENGTH s.arr`,`0n`,`s`] assume_tac array_get_aux_Success >>
+  rw[]
+QED
+
+Theorem quicksort_Success:
+  ∀ cmp l s .
+    strict_weak_order cmp
+  ⇒ ∃ l' s' . quicksort cmp l s = (Success l', s')
+Proof
+  rw[] >> Cases_on `l` >> simp[quicksort_def] >>
+  fs[ml_monadBaseTheory.st_ex_bind_def, ml_monadBaseTheory.st_ex_return_def,
+     ml_monadBaseTheory.st_ex_ignore_bind_def] >>
+  fs[fetch "-" "alloc_arr_def", ml_monadBaseTheory.Marray_alloc_def] >>
+  qspecl_then [`h::t`, `<|arr := h::REPLICATE (LENGTH t) h|>`]
+    assume_tac array_set_Success >> fs[] >>
+  qspecl_then [`cmp`,`0n`,`LENGTH t`,`s'`] assume_tac quicksort_aux_Success >>
+  rfs[] >>
+  metis_tac[array_get_Success]
+QED
+
+Theorem run_quicksort_Success:
+  ∀ cmp l . strict_weak_order cmp
+  ⇒ ∃ l' . (run_quicksort l cmp = (Success l'))
+Proof
+  fs[run_quicksort_def, fetch "-" "run_init_state_def"] >>
+  fs[ml_monadBaseTheory.run_def] >> rw[] >>
+  drule quicksort_Success >>
+  rw[] >>
+  first_x_assum (qspecl_then [`l`,`state_refs []`] mp_tac) >> rw[] >>
+  fs[]
+QED
+
+val qsort_def = Define `
+  qsort cmp l = case run_quicksort l cmp of Success result => result
+`
+val qsort_v_thm = translate qsort_def;
+
+val qsort_v_precond = Q.prove(
+  `∀ cmp l . strict_weak_order cmp ⇒ qsort_side cmp l`,
+  rw[fetch "-" "qsort_side_def"] >>
+  metis_tac[run_quicksort_Success]
+)
+
+(* TODO update precondition doesn't seem to work here
+val _ = qsort_v_precond |> update_precondition
+*)
+val qsort_v_thm = qsort_v_thm |> DISCH_ALL |>
+                  REWRITE_RULE [ml_translatorTheory.PRECONDITION_def] |>
+                  (fn th => HO_MATCH_MP th
+                    (qsort_v_precond |> SPEC_ALL |> UNDISCH_ALL)) |>
+                  DISCH_ALL
+
+val _ = save_thm("qsort_v_thm", qsort_v_thm)
 
 
 (******************************************************************************)
